examples/Engine/Requirements.thy
@@ -26,7 +26,7 @@ always2_part (\<lambda> s1. getVarBool s1 v_ignition' = False \<and> getVarBool 
    (\<lambda> s2. getVarBool s2 v_sound' = False) s"
 
 definition R6 where "R6 s \<equiv>
-always_part (\<lambda> s1. getVarBool s1 v_liquidLevel' = v_HIGH' \<longrightarrow> getVarBool s1 v_sound' = False) s"
+always2_part (\<lambda> s1. getVarBool s1 v_ignition' = True) (\<lambda> s2. getVarBool s2 v_liquidLevel' = v_HIGH') (\<lambda> s2. getVarBool s2 v_sound' = False) s"
 
 definition R7 where "R7 s \<equiv>
 P1_1_part v_WARN_LIQUID_LACK_TIMEOUT'TIMEOUT (\<lambda> s1. getVarBool s1 v_liquidLevel' = v_LOW') 
@@ -35,10 +35,27 @@ P1_1_part v_WARN_LIQUID_LACK_TIMEOUT'TIMEOUT (\<lambda> s1. getVarBool s1 v_liqu
 
 definition R8 where "R8 s \<equiv>
 always2_part (\<lambda> s1. getVarBool s1 v_ignition' = True \<and> getVarBool s1 v_onOffButton' = v_NOT_PRESSED') 
-  (\<lambda> s2. getVarBool s2 v_onOffButton' = v_PRESSED' \<and>  getVarBool s2 v_liquidLevel' = v_HIGH') 
+  (\<lambda> s2. getVarBool s2 v_onOffButton' = v_PRESSED' \<and>  getVarBool s2 v_speed' = v_LOW') 
   (\<lambda> s2. getVarBool s2 v_ignition' = False) s"
 
 definition R10 where "R10 s \<equiv>
 P1_2_part v_EMERGENCY_STOP_TIME'TIMEOUT (\<lambda> s1. getVarBool s1 v_ignition' = True \<and> getVarBool s1 v_onOffButton' = v_NOT_PRESSED') 
   (\<lambda> s2. getVarBool s2 v_onOffButton' = v_PRESSED') (\<lambda> s3. getVarBool s3 v_ignition' = True \<and> getVarBool s3 v_onOffButton' = v_PRESSED')
   (\<lambda> s4. getVarBool s4 v_ignition' = False \<or> getVarBool s4 v_onOffButton' = v_NOT_PRESSED') s"
+
+definition R11a where "R11a s \<equiv>
+P1_2_part v_SOUND_TIME'TIMEOUT (\<lambda> s1. getVarBool s1 v_ignition' = False \<and> getVarBool s1 v_onOffButton' = v_NOT_PRESSED')
+  (\<lambda> s2. getVarBool s2 v_onOffButton' = v_PRESSED' \<and> getVarBool s2 v_liquidLevel' = v_LOW')
+  (\<lambda> s3. getVarBool s3 v_sound' = True \<and> \<not> (getVarBool s3 v_liquidLevel' = v_LOW' \<and>
+    (let s2 = pred s3 in toEnvP s2 \<and> getVarBool s2 v_onOffButton' = v_NOT_PRESSED' \<and> getVarBool s3 v_onOffButton' = v_PRESSED')))
+  (\<lambda> s4. getVarBool s4 v_sound' = False \<or> (getVarBool s4 v_liquidLevel' = v_LOW' \<and>
+    (let s3 = pred s4 in toEnvP s3 \<and> getVarBool s3 v_onOffButton' = v_NOT_PRESSED' \<and> getVarBool s4 v_onOffButton' = v_PRESSED'))) s"
+
+definition R11b where "R11b s \<equiv>
+P4_2_part v_SOUND_TIME'TIMEOUT (\<lambda> s1. getVarBool s1 v_ignition' = False \<and> getVarBool s1 v_onOffButton' = v_NOT_PRESSED')
+  (\<lambda> s2. getVarBool s2 v_onOffButton' = v_PRESSED' \<and> getVarBool s2 v_liquidLevel' = v_LOW')
+(\<lambda> s3. getVarBool s3 v_sound' = True) (\<lambda> s4. getVarBool s4 v_ignition' = True) s"
+
+definition R12 where "R12 s \<equiv>
+always_part 
+  (\<lambda> s1. getVarBool s1 v_ignition' = True \<and> getVarBool s1 v_liquidLevel' = v_HIGH' \<and> getVarBool s1 v_Thigh' = True \<longrightarrow> getVarBool s1 v_valve' = True) s"
